ExistentialRules/ChaseSequence/CoreChase/Termination.lean
@@ -26,19 +26,19 @@ namespace CoreChaseBranch
   def terminates (cb : CoreChaseBranch kb) : Prop :=
     ∃ n, (cb.branch.infinite_list n = none)
 
-  def terminates_at_step (cb : CoreChaseBranch kb) (n : Nat) : Prop :=
+  def terminatesAtStep (cb : CoreChaseBranch kb) (n : Nat) : Prop :=
     (cb.branch.infinite_list n) ≠ none ∧ (cb.branch.infinite_list (n+1) = none)
 
   def terminates' (cb : CoreChaseBranch kb) : Prop :=
-    ∃ n, terminates_at_step cb n
+    ∃ n, terminatesAtStep cb n
 
   @[grind .]
-  theorem terminatesIfTerminates' (cb : CoreChaseBranch kb) : cb.terminates' → cb.terminates := by
+  theorem terminates_if_terminates' (cb : CoreChaseBranch kb) : cb.terminates' → cb.terminates := by
     intro ⟨n, a, b⟩
     exists (n + 1)
 
   @[grind .]
-  theorem terminates'IfTerminatesAndNonEmpty (cb : CoreChaseBranch kb) (non_empty : ∃ m, (cb.branch.infinite_list m).isSome) : cb.terminates → cb.terminates' := by
+  theorem terminates'_if_terminates_non_empty (cb : CoreChaseBranch kb) (non_empty : ∃ m, (cb.branch.infinite_list m).isSome) : cb.terminates → cb.terminates' := by
     intro ⟨n, a⟩
     rcases non_empty with ⟨m, c⟩
     -- n yielded from terminates, thus (n ≥ m)
@@ -61,12 +61,12 @@ namespace CoreChaseBranch
         grind
         have x : n = (n' + m) + 1 := by grind
         exists n' + m
-        unfold terminates_at_step
+        unfold terminatesAtStep
         constructor
         exact case
         grind
 
-  def last_element_index_rec  (cb : CoreChaseBranch kb) (ter' : cb.terminates') (n : Nat) : Nat :=
+  def lastElementIndexRec  (cb : CoreChaseBranch kb) (ter' : cb.terminates') (n : Nat) : Nat :=
     match eq : cb.branch.infinite_list n with
       | none => n - 1
       | some cn =>
@@ -84,24 +84,24 @@ namespace CoreChaseBranch
               subst n_max
               rw [Option.isSome_eq_isSome.mp rfl] at y
               have := cb.branch.no_holes' (Classical.choose ter' + 1) y
-              have := all_prev_some_if_is_some cb n (by exact Option.isSome_of_mem eq) m leq
+              have := leq_some_if_some cb n (by exact Option.isSome_of_mem eq) m leq
               exact Option.isSome_iff_ne_none.mp this
             apply lt_is_some (n_max + 1)
             exact gt
             exact not_none.right
           exact Nat.lt_add_one_of_le lt
-        last_element_index_rec cb ter' (n+1)
+        lastElementIndexRec cb ter' (n+1)
       termination_by Classical.choose ter' + 1 - n
 
-  def last_element_index (cb : CoreChaseBranch kb) (ter' : cb.terminates') : Nat := last_element_index_rec cb ter' 0
+  def lastElementIndex (cb : CoreChaseBranch kb) (ter' : cb.terminates') : Nat := lastElementIndexRec cb ter' 0
 
   @[grind .]
-  theorem last_element_index_eq_termintes'_index_leq (cb : CoreChaseBranch kb) (n : Nat) (term_at_n : cb.terminates_at_step n) : ∀ m, m ≤ n → last_element_index_rec cb (by exists n) m = n := by
+  theorem lastElementIndex_eq_terminatesAtStep_index_leq (cb : CoreChaseBranch kb) (n : Nat) (term_at_n : cb.terminatesAtStep n) : ∀ m, m ≤ n → lastElementIndexRec cb (by exists n) m = n := by
     intro m m_leq
-    have ter : cb.terminates := terminatesIfTerminates' cb (Exists.intro n term_at_n)
+    have ter : cb.terminates := terminates_if_terminates' cb (Exists.intro n term_at_n)
     rcases term_at_n with ⟨lhs, rhs⟩
     have ter' : cb.terminates' := Exists.intro n ⟨lhs, rhs⟩
-    unfold last_element_index_rec
+    unfold lastElementIndexRec
     induction d : (n - m) generalizing m with
       | zero =>
         have eq : m = n := by grind
@@ -109,7 +109,7 @@ namespace CoreChaseBranch
         split
         next => contradiction
         next =>
-          unfold last_element_index_rec
+          unfold lastElementIndexRec
           split
           next => simp
           next x cn heq =>
@@ -121,41 +121,41 @@ namespace CoreChaseBranch
         split
         next => grind
         next x cn heq =>
-          unfold last_element_index_rec
+          unfold lastElementIndexRec
           rw [ih]
 
   @[grind .]
-  theorem last_element_index_eq_termintes'_index (cb : CoreChaseBranch kb) (n : Nat) (term_at_n : cb.terminates_at_step n) : last_element_index cb (by exists n) = n := by
-    apply last_element_index_eq_termintes'_index_leq
+  theorem lastElementIndex_eq_terminatesAtStep_eq (cb : CoreChaseBranch kb) (n : Nat) (term_at_n : cb.terminatesAtStep n) : lastElementIndex cb (by exists n) = n := by
+    apply lastElementIndex_eq_terminatesAtStep_index_leq
     exact term_at_n
     exact Nat.zero_le n
 
   @[grind .]
-  theorem terminates'_at_last_index_ter' (cb : CoreChaseBranch kb) (ter' : cb.terminates') : cb.terminates_at_step (last_element_index cb ter') := by
+  theorem terminatesAtStep_lastElementIndex (cb : CoreChaseBranch kb) (ter' : cb.terminates') : cb.terminatesAtStep (lastElementIndex cb ter') := by
     rcases ter' with ⟨n, is_some, is_none⟩
     grind
 
   @[grind .]
-  theorem last_index_is_some (cb : CoreChaseBranch kb) (ter' : cb.terminates') : cb.branch.infinite_list (cb.last_element_index ter') ≠ none := by
+  theorem some_at_lastElementIndex (cb : CoreChaseBranch kb) (ter' : cb.terminates') : cb.branch.infinite_list (cb.lastElementIndex ter') ≠ none := by
     rcases ter' with ⟨n, term_at_n⟩
-    have := last_element_index_eq_termintes'_index cb n term_at_n
+    have := lastElementIndex_eq_terminatesAtStep_eq cb n term_at_n
     rw [this]
     exact term_at_n.left
 
-  def last_node (cb : CoreChaseBranch kb) (ter' : cb.terminates') : CoreChaseNode kb.rules :=
-      have := last_index_is_some cb ter'
-    (cb.branch.infinite_list (last_element_index cb ter')).get (by
+  def lastNode (cb : CoreChaseBranch kb) (ter' : cb.terminates') : CoreChaseNode kb.rules :=
+      have := some_at_lastElementIndex cb ter'
+    (cb.branch.infinite_list (lastElementIndex cb ter')).get (by
       exact Option.isSome_iff_ne_none.mpr this
       )
 
   def result (cb : CoreChaseBranch kb) (ter' : cb.terminates') : FactSet sig :=
-    ((cb.branch.infinite_list (last_element_index cb ter')).get (by
-      have := last_index_is_some cb ter'
+    ((cb.branch.infinite_list (lastElementIndex cb ter')).get (by
+      have := some_at_lastElementIndex cb ter'
       exact Option.isSome_iff_ne_none.mpr this
       )).core
 
   @[grind .]
-  theorem terminating_eq_index (cb : CoreChaseBranch kb) (m n : Nat) : ((cb.branch.infinite_list n) ≠ none ∧ (cb.branch.infinite_list (n+1) = none) ∧ (cb.branch.infinite_list m) ≠ none ∧ (cb.branch.infinite_list (m+1) = none)) → m = n := by
+  theorem terminating_index_eq (cb : CoreChaseBranch kb) (m n : Nat) : ((cb.branch.infinite_list n) ≠ none ∧ (cb.branch.infinite_list (n+1) = none) ∧ (cb.branch.infinite_list m) ≠ none ∧ (cb.branch.infinite_list (m+1) = none)) → m = n := by
     rintro ⟨h1, h2, h3, h4⟩
     apply Classical.byContradiction
     intro contra
@@ -194,7 +194,7 @@ namespace CoreChaseBranch
         grind
 
   @[grind .]
-  theorem terminating_has_last_index_core (cb : CoreChaseBranch kb) : cb.terminates ↔ ∃ n, (cb.branch.infinite_list n) ≠ none ∧ ∀ m, m > n -> cb.branch.infinite_list m = none := by
+  theorem terminating_has_last_index (cb : CoreChaseBranch kb) : cb.terminates ↔ ∃ n, (cb.branch.infinite_list n) ≠ none ∧ ∀ m, m > n -> cb.branch.infinite_list m = none := by
   unfold CoreChaseBranch.terminates
   constructor
   . intro h
@@ -226,46 +226,46 @@ namespace CoreChaseBranch
     simp only [gt_iff_lt, Nat.lt_add_one]
 
   @[grind .]
-  theorem exLastNodeOfTerminatingCoreChaseBranch (cb : CoreChaseBranch kb) (ter' : cb.terminates') : ∃ cn, cn = cb.last_node ter' := by
-    exists cb.last_node ter'
+  theorem ex_lastNode_if_terminates' (cb : CoreChaseBranch kb) (ter' : cb.terminates') : ∃ cn, cn = cb.lastNode ter' := by
+    exists cb.lastNode ter'
 
   @[grind .]
-  theorem exResultOfTerminatingCoreChaseBranch (cb : CoreChaseBranch kb) (ter' : cb.terminates') : ∃ fs, fs = cb.result ter' := by
+  theorem ex_result_if_terminates' (cb : CoreChaseBranch kb) (ter' : cb.terminates') : ∃ fs, fs = cb.result ter' := by
     exists cb.result ter'
 
   @[grind .]
-  theorem coreChaseResultIsCore (cb : CoreChaseBranch kb) (ter' : cb.terminates') : (cb.result ter').isWeakCore := by
+  theorem result_isWeakCore (cb : CoreChaseBranch kb) (ter' : cb.terminates') : (cb.result ter').isWeakCore := by
     unfold CoreChaseBranch.result
-    have : ∃ cn, cn = cb.last_node ter' := by exact exLastNodeOfTerminatingCoreChaseBranch cb ter'
+    have : ∃ cn, cn = cb.lastNode ter' := by exact ex_lastNode_if_terminates' cb ter'
     rcases this with ⟨cn, cn_last⟩
-    unfold CoreChaseBranch.last_node at cn_last
+    unfold lastNode at cn_last
     rw [← cn_last]
     rcases cn with ⟨_,_,_,is_core,_,_,_⟩
     exact is_core
 
   @[grind .]
-    theorem all_succ_of_last_index_none (cb : CoreChaseBranch kb) (n : Nat) (term_at_n : cb.terminates_at_step n) : ∀ m, m > n → cb.branch.infinite_list m = none := by
+    theorem gt_of_terminatesAtStep_index_none (cb : CoreChaseBranch kb) (n : Nat) (term_at_n : cb.terminatesAtStep n) : ∀ m, m > n → cb.branch.infinite_list m = none := by
       intro m gt
       rcases term_at_n with ⟨is_some, is_none⟩
       grind
 
   @[grind .]
-  theorem exLastNodeWithLastIndexIfTerminates' (cb : CoreChaseBranch kb) (ter' : cb.terminates') : ∃ last_cn, cb.branch.infinite_list (cb.last_element_index ter') = some last_cn := by
-    exists cb.last_node ter'
-    unfold last_node
+  theorem ex_lastNode_at_lastElementIndex_if_terminates' (cb : CoreChaseBranch kb) (ter' : cb.terminates') : ∃ last_cn, cb.branch.infinite_list (cb.lastElementIndex ter') = some last_cn := by
+    exists cb.lastNode ter'
+    unfold lastNode
     exact Option.eq_some_of_isSome (by
-      have := last_index_is_some cb ter'
+      have := some_at_lastElementIndex cb ter'
       exact Option.isSome_iff_ne_none.mpr this
       )
 
-  theorem neqTerminates'IfCbAllSome (cb : CoreChaseBranch kb) : (∀ (n : Nat), (cb.branch.infinite_list n).isSome) → ¬ cb.terminates' := by
+  theorem neq_terminates'_if_all_some (cb : CoreChaseBranch kb) : (∀ (n : Nat), (cb.branch.infinite_list n).isSome) → ¬ cb.terminates' := by
     intro all_some ⟨n, ⟨n_some, n_succ_none⟩⟩
     specialize all_some (n + 1)
     rw [Option.isSomeIffNeqNone] at all_some
     contradiction
 
   @[grind .]
-  theorem neqTerminatesIffCbAllSome (cb : CoreChaseBranch kb) : (∀ (n : Nat), (cb.branch.infinite_list n).isSome) ↔ ¬ cb.terminates := by
+  theorem neq_terminates_iff_all_some (cb : CoreChaseBranch kb) : (∀ (n : Nat), (cb.branch.infinite_list n).isSome) ↔ ¬ cb.terminates := by
     constructor
     intro all_some ⟨n, n_none⟩
     specialize all_some n
@@ -279,41 +279,34 @@ namespace CoreChaseBranch
     rw [Option.isSomeIffNeqNone]
     exact n_ter
 
-
   -- this one or the one below this is superfluous
-  theorem result_finite_if_cb_terminates2 (cb : CoreChaseBranch kb) (ter' : cb.terminates') : Set.finite (cb.result ter') := by
-    have : ∃ cn, cn = cb.last_node ter' := by exact exLastNodeOfTerminatingCoreChaseBranch cb ter'
+  @[grind .]
+  theorem result_finite_if_terminates' (cb : CoreChaseBranch kb) (ter' : cb.terminates') : Set.finite (cb.result ter') := by
+    have : ∃ cn, cn = cb.lastNode ter' := by exact ex_lastNode_if_terminates' cb ter'
     rcases this with ⟨cn, cn_eq⟩
     rcases ter' with ⟨n, term_at_n⟩
-    exact CoreChaseNode.all_core_finite ((cb.branch.infinite_list (cb.last_element_index (Exists.intro n term_at_n))).get (by
-      have := last_index_is_some cb (Exists.intro n term_at_n)
-      exact Option.isSome_iff_ne_none.mpr this
+    exact CoreChaseNode.core_finite ((cb.branch.infinite_list (cb.lastElementIndex (Exists.intro n term_at_n))).get (by
+      have := lastElementIndex cb (Exists.intro n term_at_n)
+      exact Option.isSome_iff_ne_none.mpr (some_at_lastElementIndex cb (Exists.intro n term_at_n))
       ))
 
   @[grind .]
-  theorem result_finite_if_cb_terminates (cb : CoreChaseBranch kb) (ter' : cb.terminates') : Set.finite (cb.result ter') := by
-    have : ∃ cn, cn = cb.last_node ter' := by exact exLastNodeOfTerminatingCoreChaseBranch cb ter'
-    rcases this with ⟨cn, cn_eq⟩
-    unfold last_node at cn_eq
-    exact result_finite_if_cb_terminates2 cb ter'
-
-  @[grind .]
-  theorem resultIsSome (cb : CoreChaseBranch kb) (ter' : cb.terminates') : cb.branch.infinite_list (cb.last_element_index ter') = some (cb.last_node ter') := by
-    unfold last_element_index last_node
+  theorem result_isSome (cb : CoreChaseBranch kb) (ter' : cb.terminates') : cb.branch.infinite_list (cb.lastElementIndex ter') = some (cb.lastNode ter') := by
+    unfold lastElementIndex lastNode
     exact Option.eq_some_of_isSome (by
-      have := last_index_is_some cb ter'
+      have := some_at_lastElementIndex cb ter'
       exact Option.isSome_iff_ne_none.mpr this
       )
 
   @[grind .]
-  theorem exHomResultIfIsSome (cb : CoreChaseBranch kb) (ter' : cb.terminates') (m : Nat) (cn cn_res : CoreChaseNode kb.rules)
-    (cn_eq : cn ∈ cb.branch.get? m) (cn_res_eq : cn_res ∈ cb.branch.get? (cb.last_element_index ter')) :
+  theorem ex_hom_result_if_isSome (cb : CoreChaseBranch kb) (ter' : cb.terminates') (m : Nat) (cn cn_res : CoreChaseNode kb.rules)
+    (cn_eq : cn ∈ cb.branch.get? m) (cn_res_eq : cn_res ∈ cb.branch.get? (cb.lastElementIndex ter')) :
       ∃ (h : GroundTermMapping sig), h.isHomomorphism cn.fs cn_res.core := by
         rcases ter' with ⟨n, term_at_n⟩
-        have ter'_eq : cb.last_element_index (Exists.intro n term_at_n : ∃ n, cb.terminates_at_step n) = n := last_element_index_eq_termintes'_index cb n term_at_n
+        have ter'_eq : cb.lastElementIndex (Exists.intro n term_at_n : ∃ n, cb.terminatesAtStep n) = n := lastElementIndex_eq_terminatesAtStep_eq cb n term_at_n
         simp only [ter'_eq] at cn_res_eq
         by_cases case : m < n
-        · have := exHomCoreAllFollowingCore cb m cn cn_eq
+        · have := ex_hom_core_geq_core cb m cn cn_eq
           specialize this (n - m)
           have eq : m + (n - m) = n := by grind
           rw [← eq] at cn_res_eq
@@ -323,22 +316,20 @@ namespace CoreChaseBranch
           exists (gtm_cn_core_cn_res_core ∘ gtm_cn_fs_cn_core)
           exact GroundTermMapping.isHomomorphism_compose gtm_cn_fs_cn_core gtm_cn_core_cn_res_core cn.fs
               cn.core cn_res.core gtm_cn_fs_cn_core_hom gtm_cn_core_cn_res_core_hom
-
         · have case : m = n ∨ m > n:= Nat.eq_or_lt_of_not_lt case
           cases case with
             | inl eq =>
               have : cn = cn_res := by grind
               rw [this]
-              exact exHomFsCore cb n cn_res cn_res_eq
+              exact ex_hom_fs_core cb n cn_res cn_res_eq
             | inr gt =>
-              have contra := CoreChaseBranch.last_element_index_eq_termintes'_index_leq cb n term_at_n m
-              unfold CoreChaseBranch.last_element_index at ter'_eq
-              have := all_succ_of_last_index_none cb n term_at_n m gt
+              have contra := lastElementIndex_eq_terminatesAtStep_index_leq cb n term_at_n m
+              unfold lastElementIndex at ter'_eq
+              have := gt_of_terminatesAtStep_index_none cb n term_at_n m gt
               grind
 
-
   @[grind .]
-  theorem cbNoneAfterLastIndex (cb : CoreChaseBranch kb) (ter' : cb.terminates') : cb.branch.infinite_list ((cb.last_element_index ter') + 1) = none := by
+  theorem succ_lastElementIndex_is_none (cb : CoreChaseBranch kb) (ter' : cb.terminates') : cb.branch.infinite_list ((cb.lastElementIndex ter') + 1) = none := by
     apply Classical.byContradiction
     rcases ter' with ⟨n_ter, n_ter_at⟩
     intro contra
@@ -349,10 +340,10 @@ namespace CoreChaseBranch
         grind
 
   @[grind .]
-  theorem cbDbSubsetResult (cb : CoreChaseBranch kb) (ter' : cb.terminates') : (kb.db.toFactSet.val ⊆ cb.result ter') := by
+  theorem db_sub_result (cb : CoreChaseBranch kb) (ter' : cb.terminates') : (kb.db.toFactSet.val ⊆ cb.result ter') := by
     let init_node := (cb.branch.infinite_list 0).get (Option.isSome_of_mem cb.database_first)
-    rcases (exLastNodeWithLastIndexIfTerminates' cb ter') with ⟨last_node, last_node_eq⟩
-    have t := cb.cbDbInAllSucc (cb.last_element_index ter') init_node last_node (Option.get_mem (Option.isSome_of_mem cb.database_first))
+    rcases (ex_lastNode_at_lastElementIndex_if_terminates' cb ter') with ⟨last_node, last_node_eq⟩
+    have t := cb.db_fs_sub_geq_core (cb.lastElementIndex ter') init_node last_node (Option.get_mem (Option.isSome_of_mem cb.database_first))
     intro f f_in
     let := cb.database_first
     have eq : init_node.fs = kb.db.toFactSet.val := by
@@ -365,10 +356,10 @@ namespace CoreChaseBranch
     simp_all
 
   @[grind .]
-  theorem coreChaseResultModelsKb (cb : CoreChaseBranch kb) (ter' : cb.terminates') : (cb.result ter').modelsKb kb := by
+  theorem result_ModelsKb (cb : CoreChaseBranch kb) (ter' : cb.terminates') : (cb.result ter').modelsKb kb := by
     constructor
     intro f f_in
-    have := cb.cbDbSubsetResult ter'
+    have := cb.db_sub_result ter'
     exact this f f_in
 
     intro r r_in gs sub
@@ -386,11 +377,11 @@ namespace CoreChaseBranch
     have trg_act : trg.active (cb.result ter') := by
       unfold Trigger.active
       exact not_imp.mp fun a => subs_not_obsolete (a sub)
-    have ex_next_node := CoreChaseBranch.exNextNodeIfExActiveTrigger cb (cb.last_element_index ter') (cb.last_node ter') (resultIsSome cb ter') ⟨trg, r_in⟩ trg_act
+    have ex_next_node := cb.ex_next_if_ex_active_trigger (cb.lastElementIndex ter') (cb.lastNode ter') (result_isSome cb ter') ⟨trg, r_in⟩ trg_act
 
     rcases ex_next_node with ⟨cn_contra,  cn_contra_eq⟩
-    have t1 := cbNoneAfterLastIndex cb ter'
-    have : cb.branch.infinite_list (cb.last_element_index ter' + 1) = some cn_contra := Option.mem_def.mp cn_contra_eq
+    have t1 := succ_lastElementIndex_is_none cb ter'
+    have : cb.branch.infinite_list (cb.lastElementIndex ter' + 1) = some cn_contra := Option.mem_def.mp cn_contra_eq
     rw [t1] at this
     contradiction
 
