ExistentialRules/ChaseSequence/CoreChase/CoreChaseNode.lean
@@ -42,7 +42,7 @@ namespace CoreChaseNode
     exact Set.finite_of_subset_finite fs_fin sub
 
   @[grind .]
-  theorem all_core_finite (node : CoreChaseNode kb.rules) : Set.finite (node.core) := by
+  theorem core_finite (node : CoreChaseNode kb.rules) : Set.finite (node.core) := by
     apply CoreChaseNode.core_finite_if_fs_finite
     exact node.fs_fin
 
