ExistentialRules/ChaseSequence/CoreChase/Homomorphisms.lean
@@ -23,21 +23,21 @@ namespace CoreChaseBranch
 
 
   @[grind .]
-  theorem exHomFsCore (cb : CoreChaseBranch kb) (n : Nat) (x : CoreChaseNode kb.rules) (x_eq : x ∈ cb.branch.get? n) :
+  theorem ex_hom_fs_core (cb : CoreChaseBranch kb) (n : Nat) (x : CoreChaseNode kb.rules) (x_eq : x ∈ cb.branch.get? n) :
     ∃ (h : GroundTermMapping sig), h.isHomomorphism x.fs x.core := by
       exact x.core_sse.right
 
   @[grind .]
-  theorem exHomPrevCoreToFactSet (cb : CoreChaseBranch kb) (n : Nat) (x y : CoreChaseNode kb.rules)
+  theorem ex_hom_prev_core_next_fs (cb : CoreChaseBranch kb) (n : Nat) (x y : CoreChaseNode kb.rules)
     (x_eq : x ∈ cb.branch.get? n) (y_eq : y ∈ cb.branch.get? (n + 1)) : ∃ (h : GroundTermMapping sig), h.isHomomorphism x.core y.fs := by
       have sub : x.core ⊆ y.fs := before_core_sub_after_fs cb n x y x_eq y_eq
-      have := x.core.exHomSubToSet y.fs sub
+      have := x.core.ex_hom_sub y.fs sub
       exact this
 
   @[grind .]
-  theorem exGtmHomSubsetFsCore (cb : CoreChaseBranch kb) (cn : CoreChaseNode kb.rules) (n : Nat) (cn_eq : cn ∈ cb.branch.get? n) :
+  theorem ex_hom_applyFactSet_fs_core (cb : CoreChaseBranch kb) (cn : CoreChaseNode kb.rules) (n : Nat) (cn_eq : cn ∈ cb.branch.get? n) :
     ∃ (gtm : GroundTermMapping sig), gtm.applyFactSet cn.fs ⊆ cn.core := by
-      rcases (exHomFsCore cb n cn cn_eq) with ⟨gtm, gtm_hom⟩
+      rcases (ex_hom_fs_core cb n cn cn_eq) with ⟨gtm, gtm_hom⟩
       exists gtm
       intro f f_in
       unfold GroundTermMapping.applyFactSet at f_in
@@ -48,22 +48,22 @@ namespace CoreChaseBranch
       exact ahl
 
   @[grind .]
-  theorem exHomCoreSuccCoreIfSuccIsSome (cb : CoreChaseBranch kb) (n : Nat) (x y : CoreChaseNode kb.rules)
+  theorem ex_hom_core_succ_core_if_some (cb : CoreChaseBranch kb) (n : Nat) (x y : CoreChaseNode kb.rules)
     (x_eq : cb.branch.infinite_list n = some x) (y_eq : cb.branch.infinite_list (n + 1) = some y) :
       ∃ (h : GroundTermMapping sig), h.isHomomorphism x.core y.core := by
       have y_core := y.core_sse
       rcases y_core with ⟨sub, ⟨gtm_yfs_ycore, gtm_yfs_ycore_hom⟩⟩
-      have : ∃ (h : GroundTermMapping sig), h.isHomomorphism x.core y.fs := exHomPrevCoreToFactSet cb n x y x_eq y_eq
+      have : ∃ (h : GroundTermMapping sig), h.isHomomorphism x.core y.fs := ex_hom_prev_core_next_fs cb n x y x_eq y_eq
       rcases this with ⟨gtm_xcore_yfs, gtm_xcore_yfs_hom⟩
       exists (gtm_yfs_ycore ∘ gtm_xcore_yfs)
       exact GroundTermMapping.isHomomorphism_compose gtm_xcore_yfs gtm_yfs_ycore x.core y.fs y.core gtm_xcore_yfs_hom gtm_yfs_ycore_hom
 
   @[grind .]
-  theorem exHomFsSuccFsIfSuccIsSome (cb : CoreChaseBranch kb) (n : Nat) (x y : CoreChaseNode kb.rules)
+  theorem ex_hom_fs_succ_fs_if_some (cb : CoreChaseBranch kb) (n : Nat) (x y : CoreChaseNode kb.rules)
     (x_eq : cb.branch.infinite_list n = some x) (y_eq : cb.branch.infinite_list (n + 1) = some y) :
       ∃ (h : GroundTermMapping sig), h.isHomomorphism x.fs y.fs := by
         have x_core := x.core_sse
-        have : ∃ (h : GroundTermMapping sig), h.isHomomorphism x.core y.fs := exHomPrevCoreToFactSet cb n x y x_eq y_eq
+        have : ∃ (h : GroundTermMapping sig), h.isHomomorphism x.core y.fs := ex_hom_prev_core_next_fs cb n x y x_eq y_eq
         rcases this with ⟨gtm_xcore_yfs, gtm_xcore_yfs_hom⟩
         rcases x_core with ⟨sub, gtm_xfs_xcore, gtm_xfs_xcore_hom⟩
         exists (gtm_xcore_yfs ∘ gtm_xfs_xcore)
@@ -71,7 +71,7 @@ namespace CoreChaseBranch
 
   -- t16 (A_0 → A_1 → A_2 → ...)
   @[grind .]
-  theorem exHomCoreAllFollowingCore (cb : CoreChaseBranch kb) (n : Nat) (x : CoreChaseNode kb.rules) (x_eq : x ∈ cb.branch.get? n) :
+  theorem ex_hom_core_geq_core (cb : CoreChaseBranch kb) (n : Nat) (x : CoreChaseNode kb.rules) (x_eq : x ∈ cb.branch.get? n) :
       ∀ m, ∀ y, y ∈ cb.branch.get? (n + m) → ∃ (h : GroundTermMapping sig), h.isHomomorphism x.core y.core := by
       intro m
       induction m with
@@ -92,14 +92,14 @@ namespace CoreChaseBranch
         rcases ex_cm with ⟨z, z_eq⟩
         specialize ih z z_eq
         rcases ih with ⟨gtm_x_z, gtm_x_z_hom⟩
-        have : ∃ (h : GroundTermMapping sig), h.isHomomorphism z.core y.core := exHomCoreSuccCoreIfSuccIsSome cb (n + m) z y z_eq y_eq
+        have : ∃ (h : GroundTermMapping sig), h.isHomomorphism z.core y.core := ex_hom_core_succ_core_if_some cb (n + m) z y z_eq y_eq
         rcases this with ⟨gtm_z_y, gtm_z_y_hom⟩
         exists (gtm_z_y ∘ gtm_x_z)
         exact GroundTermMapping.isHomomorphism_compose gtm_x_z gtm_z_y x.core z.core y.core gtm_x_z_hom gtm_z_y_hom
 
   @[grind .]
   -- exHomStepToAllFollowing
-  theorem exHomFsAllFollowingFs (cb : CoreChaseBranch kb) (n : Nat) (x : CoreChaseNode kb.rules) (x_eq : x ∈ cb.branch.get? n) :
+  theorem ex_hom_fs_geq_fs (cb : CoreChaseBranch kb) (n : Nat) (x : CoreChaseNode kb.rules) (x_eq : x ∈ cb.branch.get? n) :
         ∀ m, ∀ y, y ∈ cb.branch.get? (n + m) → ∃ (h : GroundTermMapping sig), h.isHomomorphism x.fs y.fs := by
       intro m
       induction m with
@@ -115,26 +115,26 @@ namespace CoreChaseBranch
         rcases ex_z with ⟨z, z_eq⟩
         specialize ih z z_eq
         rcases ih with ⟨gtm_x_z, gtm_x_z_hom⟩
-        have ex_gtm_z_y : ∃ (h : GroundTermMapping sig), h.isHomomorphism z.fs y.fs := cb.exHomFsSuccFsIfSuccIsSome (n + m) z y z_eq y_eq
+        have ex_gtm_z_y : ∃ (h : GroundTermMapping sig), h.isHomomorphism z.fs y.fs := cb.ex_hom_fs_succ_fs_if_some (n + m) z y z_eq y_eq
         rcases ex_gtm_z_y with ⟨gtm_z_y, gtm_z_y_hom⟩
         exists (gtm_z_y ∘ gtm_x_z)
         exact GroundTermMapping.isHomomorphism_compose gtm_x_z gtm_z_y x.fs z.fs y.fs gtm_x_z_hom gtm_z_y_hom
 
   @[grind .]
-  theorem homFsToFsAlsoHomCoreToFs (fs : FactSet sig) (cn : CoreChaseNode kb.rules) (h : GroundTermMapping sig) (h_hom : h.isHomomorphism cn.fs fs) : h.isHomomorphism cn.core fs := by
+  theorem gtm_core_set_if_gtm_fs_set (fs : FactSet sig) (cn : CoreChaseNode kb.rules) (h : GroundTermMapping sig) (h_hom : h.isHomomorphism cn.fs fs) : h.isHomomorphism cn.core fs := by
     rcases h_hom with ⟨h_c, h_af⟩
     constructor
     exact h_c
     intro f f_in
     specialize h_af f
     apply h_af
-    exact GroundTermMapping.memApplyFactSetIfMemApplyFactSetSubSet h cn.core cn.fs f f_in (cn.core_sse.left)
+    exact h.mem_applyFactSet_if_mem_applyFactSet_sub cn.core cn.fs f f_in (cn.core_sse.left)
 
   @[grind .]
-  theorem gtmFsCoreIsEndo (cb : CoreChaseBranch kb) (cn : CoreChaseNode kb.rules) (n : Nat) (cn_eq : cb.branch.infinite_list n = some cn) (gtm : GroundTermMapping sig) (gtm_hom : gtm.isHomomorphism cn.fs cn.core):
+  theorem gtm_fs_core_is_endo (cb : CoreChaseBranch kb) (cn : CoreChaseNode kb.rules) (n : Nat) (cn_eq : cb.branch.infinite_list n = some cn) (gtm : GroundTermMapping sig) (gtm_hom : gtm.isHomomorphism cn.fs cn.core):
      (gtm.surjective_for_domain_and_image_set cn.core.terms cn.core.terms) := by
-      have sc := FactSet.isStrongCore_of_isWeakCore_of_finite cn.core cn.is_core (CoreChaseNode.all_core_finite cn)
-      specialize sc gtm (homFsToFsAlsoHomCoreToFs cn.core cn gtm gtm_hom)
+      have sc := FactSet.isStrongCore_of_isWeakCore_of_finite cn.core cn.is_core cn.core_finite
+      specialize sc gtm (gtm_core_set_if_gtm_fs_set cn.core cn gtm gtm_hom)
       rcases sc with ⟨s1, s2, s3⟩
       exact s3
 
